skeleton for typechecking of pcal algorithms

PlusCalCompiler/Passes/Typechecker/Monad.lean
@@ -46,35 +46,70 @@ section
 end
 
 
+/--
+  The class of monads `m` with simple context lookup capabilities.
+-/
+class MonadContext.{u, v} (α β : Type _) (m : Type u → Type v) where
+  /-- Lookup a variable in the local context, and return its entry if found. -/
+  lookupDecl : α → m (Option β)
+export MonadContext (lookupDecl)
+
+instance {α β m} [BEq α] [Hashable α] [Monad m] [MonadReader (Std.HashMap α β) m] :
+    MonadContext α β m where
+  lookupDecl x := (Std.HashMap.get? · x) <$> read
+
+instance {α β m} [BEq α] [Hashable α] [Monad m] [MonadState (Std.HashMap α β) m] :
+    MonadContext α β m where
+  lookupDecl x := (Std.HashMap.get? · x) <$> get
 
 /--
   The class of monads `m` with local context capabilites.
   `α` is the type of variable identifiers, and `β` the type of data to be registered
   for variables.
 -/
-class MonadLocalContext.{u, v} (α β : Type _) (m : Type u → Type v) where
+class MonadLocalContext.{u, v} (α β : Type _) (m : Type u → Type v) extends MonadContext α β m where
   /-- Execute an action in a local context augmented with a variable entry. -/
   withLocalDecl {γ} : α → β → m γ → m γ
-  /-- Lookup a variable in the local context, and return its entry if found. -/
-  lookupDecl : α → m (Option β)
-export MonadLocalContext (withLocalDecl lookupDecl)
+export MonadLocalContext (withLocalDecl)
 
 instance {α β m} [BEq α] [Hashable α] [Monad m] [MonadReader (Std.HashMap α β) m] [MonadWithReader (Std.HashMap α β) m] :
     MonadLocalContext α β m where
-  withLocalDecl x y act := withReader (Std.HashMap.insert · x y) act
-  lookupDecl x := (Std.HashMap.get? · x) <$> read
+  withLocalDecl x y := withReader (Std.HashMap.insert · x y)
+
+instance {α β m} [BEq α] [Hashable α] [Monad m] [MonadState (Std.HashMap α β) m] :
+    MonadLocalContext α β m where
+  withLocalDecl x y act := do
+    let σ ← modifyGet λ σ ↦ (σ, σ.insert x y)
+    act <* MonadState.set σ
+
+class MonadGlobalContext.{u, v} (α β : Type _) (m : Type u → Type v) extends MonadLocalContext α β m where
+  /-- Insert a new declaration into the global context. -/
+  addDecl : α → β → m PUnit
+export MonadGlobalContext (addDecl)
+
+instance {α β m} [BEq α] [Hashable α] [Monad m] [MonadState (Std.HashMap α β) m] :
+    MonadGlobalContext α β m where
+  addDecl x y := modify (Std.HashMap.insert · x y)
+
 
 -------------
 
-class abbrev MonadTC.{u, v} (m : Type u → Type v) :=
+class abbrev MonadTCExpr.{u, v} (m : Type u → Type v) :=
   MonadLocalContext String SurfaceTLAPlus.Typ m,
   MonadExcept TCError m,
   MonadWriter (List TCWarning) m
 
+class abbrev MonadTC.{u, v} (m : Type u → Type v) :=
+  MonadGlobalContext String SurfaceTLAPlus.Typ m,
+  MonadExcept TCError m,
+  MonadWriter (List TCWarning) m
+
+instance (priority := low) {m} [MonadTC m] : MonadTCExpr m where
+
 -------------
 
-/-- The typechecker monad. -/
-abbrev TC.{u} (α : Type u) : Type u :=
+/-- The typechecker monad, for expressions. -/
+abbrev TCExpr.{u} (α : Type u) : Type u :=
   ReaderT
     (Std.HashMap String SurfaceTLAPlus.Typ)
     (ExceptT
@@ -84,19 +119,52 @@ abbrev TC.{u} (α : Type u) : Type u :=
         Id))
     α
 
-nonrec abbrev TC.run {α} (Γ : Std.HashMap String SurfaceTLAPlus.Typ) (x : TC α) :
+nonrec abbrev TCExpr.run {α} (Γ : Std.HashMap String SurfaceTLAPlus.Typ) (x : TCExpr α) :
     Except TCError α × List TCWarning :=
   x.run Γ |>.run |>.run |>.run
+
+instance (priority := high) : Monad TCExpr := inferInstance
+
+instance (priority := high) : MonadLocalContext String SurfaceTLAPlus.Typ TCExpr := inferInstance
+
+instance (priority := high) : MonadExcept TCError TCExpr := inferInstance
+
+instance (priority := high) : MonadWriter (List TCWarning) TCExpr := inferInstance
+
+instance (priority := high) : Std.Do.WP TCExpr (.arg (Std.HashMap String SurfaceTLAPlus.Typ) <| .except TCError <| .arg (List TCWarning) .pure) :=
+  inferInstance
+
+instance (priority := high) : Std.Do.WPMonad TCExpr (.arg (Std.HashMap String SurfaceTLAPlus.Typ) <| .except TCError <| .arg (List TCWarning) .pure) :=
+  inferInstance
+
+----------------
+
+/-- The typechecker monad. -/
+abbrev TC.{u} (α : Type u) : Type u :=
+  StateT
+    (Std.HashMap String SurfaceTLAPlus.Typ)
+    (ExceptT
+      TCError
+      (WriterT
+        (List TCWarning)
+        Id))
+    α
+
+nonrec abbrev TC.run {α} (Γ : Std.HashMap String SurfaceTLAPlus.Typ) (x : TC α) :
+    Except TCError (α × Std.HashMap String SurfaceTLAPlus.Typ) × List TCWarning :=
+  x.run Γ |>.run |>.run |>.run
+
+-- def TC.ofTCExpr {α} (act : )
 
 instance (priority := high) : Monad TC := inferInstance
 
 instance (priority := high) : MonadLocalContext String SurfaceTLAPlus.Typ TC := inferInstance
 
+instance (priority := high) : MonadGlobalContext String SurfaceTLAPlus.Typ TC := inferInstance
+
 instance (priority := high) : MonadExcept TCError TC := inferInstance
 
 instance (priority := high) : MonadWriter (List TCWarning) TC := inferInstance
-
-instance : MonadTC TC := inferInstance
 
 instance (priority := high) : Std.Do.WP TC (.arg (Std.HashMap String SurfaceTLAPlus.Typ) <| .except TCError <| .arg (List TCWarning) .pure) :=
   inferInstance
